examples/pseudo_bool/cp_encoding/ilpScript.sml
@@ -5,7 +5,7 @@ Theory ilp
 Libs
   preamble
 Ancestors
-  mlint pbc cp
+  mlint pbc cp pbc_encode
 
 (*
   This "ILP"-style intermediate language is designed for convenience of
@@ -72,3 +72,186 @@ Proof
   drule norm_varcs_aux_sound>>
   simp[eval_ilin_term_def,iSUM_def]
 QED
+
+Definition min_iterm_def:
+  min_iterm bnd (c,X) =
+    let (lb,ub) = bnd X in
+      if c < 0i then c * ub
+      else c * lb
+End
+
+Theorem min_iterm_le:
+  valid_assignment bnd w ⇒
+  min_iterm bnd t ≤ eval_iterm w t
+Proof
+  Cases_on`t`>>
+  rw[valid_assignment_def,eval_iterm_def,min_iterm_def]>>
+  pairarg_tac>>gvs[]>>
+  first_x_assum drule>>gvs[]>>
+  rw[]
+  >- (
+    DEP_REWRITE_TAC[INT_LE_ANTIMONO]>>
+    simp[])
+  >>
+    match_mp_tac INT_LE_MONO_IMP>>
+    intLib.ARITH_TAC
+QED
+
+Definition min_ilin_term_def:
+  min_ilin_term bnd (xs:'a ilin_term) =
+  iSUM (MAP (min_iterm bnd) xs)
+End
+
+Theorem eval_ilin_term_min_ilin_term:
+  valid_assignment bnd w ⇒
+  min_ilin_term bnd xs ≤ eval_ilin_term w xs
+Proof
+  rw[min_ilin_term_def,eval_ilin_term_def]>>
+  match_mp_tac iSUM_MAP_le>>
+  rw[]>>
+  metis_tac[min_iterm_le]
+QED
+
+(* List of literals imply iconstraint under bounds *)
+Definition bits_imply_def:
+  bits_imply bnd xs cc =
+  case cc of (is,bs,c) =>
+    let r = c - min_ilin_term bnd is - min_lin_term bs in
+    let rr = int_max r 0 in
+    (is, MAP (λx. (rr, negate x)) xs ++ bs, c)
+End
+
+Theorem bits_imply_sem[simp]:
+  valid_assignment bnd wi ⇒
+  iconstraint_sem (bits_imply bnd xs c) (wi,wb) =
+    (EVERY (lit wb) xs ⇒ iconstraint_sem c (wi,wb))
+Proof
+  rw[bits_imply_def]>>
+  every_case_tac>>gvs[iconstraint_sem_def]>>
+  Cases_on`EVERY (lit wb) xs`
+  >- (
+    drule eval_lin_term_MAP_negate_0>> rw[])>>
+  simp[]>>
+  rename1`eval_ilin_term wi is + (_ + eval_lin_term wb bs) ≥ rr`>>
+  drule eval_ilin_term_min_ilin_term>>
+  disch_then(qspec_then`is` assume_tac)>>
+  `min_lin_term bs ≤ eval_lin_term wb bs` by
+    metis_tac[eval_lin_term_min_lin_term]>>
+  qmatch_goalsub_abbrev_tac`int_max r 0`>>
+  drule eval_lin_term_MAP_negate_ge>>
+  disch_then(qspec_then`int_max r 0` mp_tac)>>
+  impl_tac >- intLib.ARITH_TAC>>
+  rw[Abbr`r`]>>
+  intLib.ARITH_TAC
+QED
+
+Theorem eval_ilin_term_flip_coeffs[simp]:
+  eval_ilin_term w (flip_coeffs xs) = - eval_ilin_term w xs
+Proof
+  simp[eval_ilin_term_def,flip_coeffs_def]>>
+  Induct_on`xs`>>rw[iSUM_def]>>
+  pairarg_tac>>simp[]>>
+  intLib.ARITH_TAC
+QED
+
+Definition max_iterm_def:
+  max_iterm bnd (c,X) =
+    let (lb,ub) = bnd X in
+      if c < 0i then c * lb
+      else c * ub
+End
+
+Theorem max_iterm_le:
+  valid_assignment bnd w ⇒
+  eval_iterm w t ≤ max_iterm bnd t
+Proof
+  Cases_on`t`>>
+  rw[valid_assignment_def,eval_iterm_def,max_iterm_def]>>
+  pairarg_tac>>gvs[]>>rw[]>>
+  first_x_assum(qspec_then`r` mp_tac)>>gvs[]>>
+  rw[]
+  >- (
+    DEP_REWRITE_TAC[INT_LE_ANTIMONO]>>
+    simp[])
+  >>
+    match_mp_tac INT_LE_MONO_IMP>>
+    intLib.ARITH_TAC
+QED
+
+Definition max_ilin_term_def:
+  max_ilin_term bnd (xs:'a ilin_term) =
+  iSUM (MAP (max_iterm bnd) xs)
+End
+
+Theorem eval_ilin_term_max_ilin_term:
+  valid_assignment bnd w ⇒
+  eval_ilin_term w xs ≤ max_ilin_term bnd xs
+Proof
+  rw[max_ilin_term_def,eval_ilin_term_def]>>
+  match_mp_tac iSUM_MAP_le>>
+  rw[]>>
+  metis_tac[max_iterm_le]
+QED
+
+(* constraint implies list of literals *)
+Definition imply_bits_def:
+  imply_bits bnd xs cc =
+  case cc of (is,bs,c) =>
+    let nis = flip_coeffs is in
+    let nbs = flip_coeffs bs in
+    let nc = 1 - c in
+    let r = nc + max_ilin_term bnd is + max_lin_term bs in
+    let rr = int_max r 0 in
+    MAP (λx. (nis, (rr, x) :: nbs, nc)) xs
+End
+
+Theorem imply_bits_sem[simp]:
+  valid_assignment bnd wi ⇒
+  EVERY (λx. iconstraint_sem x (wi,wb)) (imply_bits bnd xs c)
+  =
+  (iconstraint_sem c (wi,wb) ⇒ EVERY (lit wb) xs)
+Proof
+  rw[imply_bits_def]>>
+  every_case_tac>>
+  gvs[EVERY_MEM,MEM_MAP,PULL_EXISTS,PULL_FORALL,iconstraint_sem_def]>>
+  ho_match_mp_tac
+    (METIS_PROVE []
+    ``
+      (∀x. (P x ⇒ (Q x ⇔ (A x ⇒ R x)))) ⇒
+      ((!x. (P x ⇒ Q x)) ⇔ (!x. (A x ⇒ P x ⇒ R x)))``)>>
+  rw[]>>
+  rename1`lit wb x`>>
+  Cases_on`lit wb x`>>simp[]
+  >- (
+    rename1`-eval_ilin_term wi is + (_ + -eval_lin_term wb bs) ≥ 1 - rr`>>
+    drule eval_ilin_term_max_ilin_term>>
+    disch_then(qspec_then`is` assume_tac)>>
+    `eval_lin_term wb bs ≤ max_lin_term bs` by
+      metis_tac[eval_lin_term_max_lin_term]>>
+    intLib.ARITH_TAC)>>
+  intLib.ARITH_TAC
+QED
+
+(* encodes iff *)
+Definition bimply_bits_def:
+  bimply_bits bnd xs cc =
+  bits_imply bnd xs cc ::
+  imply_bits bnd xs cc
+End
+
+Theorem bimply_bits_sem[simp]:
+  valid_assignment bnd wi ⇒
+  EVERY (λx. iconstraint_sem x (wi,wb)) (bimply_bits bnd xs c)
+  =
+  (iconstraint_sem c (wi,wb) ⇔ EVERY (lit wb) xs)
+Proof
+  rw[bimply_bits_def]>>
+  metis_tac[imply_bits_sem,bits_imply_sem]
+QED
+
+Theorem eval_ilin_term_NIL[simp]:
+  eval_ilin_term w [] = 0
+Proof
+  rw[eval_ilin_term_def,iSUM_def]
+QED
+
